examples/modfair/ModFairTestAIproof.v
@@ -1,0 +1,71 @@
+Require Import ModFairTest2A ModFairTest2I ModFairA ModFairNot ModFairANotproof.
+Require Import HoareDef SimModSem.
+Require Import Coqlib.
+Require Import ImpPrelude.
+Require Import Skeleton.
+Require Import PCM.
+Require Import ModSem ModSemE Behavior.
+Require Import Relation_Definitions.
+
+(*** TODO: export these in Coqlib or Universe ***)
+Require Import Relation_Operators.
+Require Import RelationPairs.
+From ITree Require Import
+     Events.MapDefault.
+From ExtLib Require Import
+     Core.RelDec
+     Structures.Maps
+     Data.Map.FMapAList.
+Require Import HTactics ProofMode IPM.
+Require Import OpenDef.
+Require Import Mem1 STB Invariant.
+
+Require Import IProofMode IRed ITactics.
+
+Require Import sProp sWorld World SRF.
+From stdpp Require Import coPset gmap namespaces.
+
+Require Import WFLibLarge FairCounter.
+From Ordinal Require Import ClassicalOrdinal.
+
+Set Implicit Arguments.
+
+Local Open Scope nat_scope.
+
+Section SIMMODSEM.
+  Context `{_W: CtxWD.t}.
+        
+  Variable GlobalStb: Sk.t -> gname -> option fspec.
+  Hypothesis STBINCL: forall sk, stb_incl (to_stb (FairStb nat)) (GlobalStb sk).
+  Hypothesis STB_fair: forall sk, (GlobalStb sk) "fair" = Some (fair_spec nat).
+
+  Definition Ist: Any.t -> Any.t -> iProp :=
+    fun st_src st_tgt => (⌜True⌝)%I.
+
+  Ltac coapply :=
+    iApply isim_progress;
+    iApply isim_base;
+    match goal with [|- context[_ _ _ _ _ (?st_src, _) (?st_tgt, _)]] =>
+      iApply ("CIH" $! (@existT _ (λ _, _) st_src st_tgt)); eauto
+    end.
+
+  Lemma simF_test:
+    forall i_src: iimap nat owf,
+    HModPair.sim_fun
+      (HMod.add (ModFairTest2A.HFair GlobalStb) (ModFairA.HFair i_src))
+      (HMod.add ModFairTest2I.Fair (ModFairA.HFair (@i_zero nat)))
+      (IstProd Ist (IstFairSrc nat)) "test".
+  Proof.
+    simF_init ModFairTest2A.HFair_unfold ModFairTest2I.Fair_unfold ModFairTest2A.testF ModFairTest2I.testF.
+  Admitted.
+  
+  Theorem sim: 
+    forall i_tgt: iimap nat nat_wf,
+      HModPair.sim 
+        (HMod.add (ModFairTest2A.HFair GlobalStb) (ModFairNot.HUnFair i_tgt (GlobalStb)))
+        (HMod.add ModFairTest2I.Fair (ModFairA.HFair i_tgt)) 
+        (IstProd Ist (IstFairTgt nat)).
+  Proof.
+  Admitted.
+
+End SIMMODSEM.
